lib+spec+proof: generalise list_queue_relation
Introduce the type head_end_ptrs to model
doubly-linked lists, and use this type within the
definition of list_queue_relation and related
definitions.

Definitions and lemmas about list_queue_relation are
now in Lib.

Compatibility with the Haskell type TcbQueue is provided
by a series of abbreviations.

Signed-off-by: Michael McInerney <michael.mcinerney@proofcraft.systems>

spec/haskell/src/SEL4/Kernel/Thread.lhs
@@ -665,7 +665,7 @@ Remove a thread from a queue, which must originally contain the thread
 
 The queue is the singleton containing tcbPtr
 
->         then return $ TcbQueue { tcbQueueHead = Nothing, tcbQueueEnd = Nothing }
+>         then return emptyQueue
 >         else
 >             if tcbQueueHead queue == Just tcbPtr
 
