spec/design/skel/Structures_H.thy
@@ -35,8 +35,30 @@ arch_requalify_consts (H)
   atcbContextGet
   atcbContextSet
 
-#INCLUDE_HASKELL SEL4/Object/Structures.lhs decls_only NOT isNullCap isUntypedCap isIRQControlCap isReplyCap isDomainCap isNotificationCap TcbFlag tcbFlagToWord tcbFlagMask
-#INCLUDE_HASKELL SEL4/Object/Structures.lhs bodies_only NOT kernelObjectTypeName isNullCap isUntypedCap isIRQControlCap isReplyCap isDomainCap isNotificationCap tcbFlagToWord tcbFlagMask
+type_synonym tcb_queue = "machine_word head_end_ptrs"
+
+abbreviation (input) tcbQueueHead :: "tcb_queue \<Rightarrow> machine_word option" where
+  "tcbQueueHead \<equiv> he_ptrs_head"
+
+abbreviation (input) tcbQueueHead_update ::
+  "(machine_word option \<Rightarrow> machine_word option) \<Rightarrow> tcb_queue \<Rightarrow> tcb_queue" where
+  "tcbQueueHead_update \<equiv> he_ptrs_head_update"
+
+abbreviation (input) tcbQueueEnd :: "tcb_queue \<Rightarrow> machine_word option" where
+  "tcbQueueEnd \<equiv> he_ptrs_end"
+
+abbreviation (input) tcbQueueEnd_update ::
+  "(machine_word option \<Rightarrow> machine_word option) \<Rightarrow> tcb_queue \<Rightarrow> tcb_queue" where
+  "tcbQueueEnd_update \<equiv> he_ptrs_end_update"
+
+abbreviation (input) emptyQueue :: tcb_queue where
+  "emptyQueue \<equiv> emptyHeadEndPtrs"
+
+abbreviation (input) tcbQueueEmpty :: "tcb_queue \<Rightarrow> bool" where
+  "tcbQueueEmpty \<equiv> headEndPtrsEmpty"
+
+#INCLUDE_HASKELL SEL4/Object/Structures.lhs decls_only NOT isNullCap isUntypedCap isIRQControlCap isReplyCap isDomainCap isNotificationCap TcbFlag tcbFlagToWord tcbFlagMask TcbQueue emptyQueue
+#INCLUDE_HASKELL SEL4/Object/Structures.lhs bodies_only NOT kernelObjectTypeName isNullCap isUntypedCap isIRQControlCap isReplyCap isDomainCap isNotificationCap tcbFlagToWord tcbFlagMask TcbQueue emptyQueue
 
 
 end
