spec/design/skel/Thread_H.thy
@@ -43,7 +43,7 @@ requalify_consts (aliasing)
 end
 end
 
-#INCLUDE_HASKELL SEL4/Kernel/Thread.lhs Arch=Arch bodies_only NOT doNormalTransfer doIPCTransfer doReplyTransfer doNormalTransfer transferCaps transferCapsToSlots
+#INCLUDE_HASKELL SEL4/Kernel/Thread.lhs Arch=Arch bodies_only NOT doNormalTransfer doIPCTransfer doReplyTransfer doNormalTransfer transferCaps transferCapsToSlots tcbQueueEmpty
 
 #INCLUDE_HASKELL SEL4/Kernel/Thread.lhs Arch=Arch ONLY transferCapsToSlots
 
